# 기초 수식

## 1번

$$
T(n) = T(n - 1) + 1 \\
T(n - 1) = T(n - 2) + 1 \\
\vdots \\
T(2) = T(1) + 1 \\
T(1) = 1 \\
\therefore T(n) = 1+\dots + 1 = O(n)
$$



## 2번

$$
T(n) = T(n - 1) + n \\
T(n - 1) = T(n - 2) + n - 1 \\
\vdots \\
T(2) = T(1) + 2 \\
T(1) = 1 \\
\therefore T(n) = n + (n - 1) + \dots +1=O(n^2)
$$



## 4번

$$
T(n) = T({n \over 2}) + 1 \\
T({n \over 2}) = T({n \over 4}) + 1 \\
\dots \ for \ \log n \ time\\ 
T(2) = T(1) + 1 \\
T(1) = 1 \\
\therefore T(n) = 1 + \dots \ for \ \log n \ time +1=O(\log n)
$$



## 6번

$$
T(n) = 2 \ T({n \over 2}) + n \\
T({n \over 2}) = 2 \ T({n \over 4}) + {n \over 2} \\
\dots \ for \ \log n \ time\\ 
T(2) = 2 \ T(1) + 2 \\
T(1) = 1 \\
\therefore T(n) = n + \dots \ for \ \log n \ time +n=O(n \log n)
$$

위의 식에 아래식을 대입할 때, 더하는 상수는 n으로 고정된다.



## 8번

$$
T(n) = T(n - 1) + {1 \over  n} \\
T(n - 1) = T(n - 2) + {1 \over n - 1} \\
\vdots \\
T(2) = T(1) + {1 \over 2} \\
T(1) = 1 \\
\therefore T(n) = {1 \over  n} + {1 \over  n - 1} +\dots + {1 \over 2} + 1 = O(\log n)
$$

[Reference for sum of 1/n](https://gateoverflow.in/41209/Find-oder-of-this-algorithm-t-n-t-n-1-1-n-if-n-1)

